Makefile
@@ -139,7 +139,8 @@ CONCUR_FILES= \
   resource_decay_join.v join_lemmas.v coqlib5.v age_to.v \
   konig.v safety.v \
   reach_lemmas.v reestablish.v ret_lemmas.v lifting.v linking_inv.v linking_spec.v call_lemmas.v \
-  machine_semantics.v machine_semantics_lemmas.v machine_simulation.v
+  machine_semantics.v machine_semantics_lemmas.v machine_simulation.v \
+  coinductive_safety.v
 
 PACO_FILES= \
   hpattern.v\
